Matroid/ForMathlib/Lattice.lean
@@ -1,0 +1,16 @@
+import Mathlib.Order.SupIndep
+
+open Set
+
+section Lattice
+
+theorem sSup_iUnion {α ι : Type*} [CompleteLattice α] {s : ι → Set α} :
+    sSup (⋃ i, s i) = iSup (fun i ↦ sSup (s i)) := by
+  simp only [le_antisymm_iff, sSup_le_iff, mem_iUnion, forall_exists_index, iSup_le_iff]
+  exact ⟨fun a i h ↦ le_iSup_of_le i <| le_sSup h, fun i a h ↦ le_sSup <| mem_iUnion_of_mem i h⟩
+
+@[simp] theorem setIndependent_singleton {α : Type*} [CompleteLattice α] (s : α) :
+    CompleteLattice.SetIndependent {s} := by
+  simp [CompleteLattice.SetIndependent]
+
+end Lattice
